# HW1015byJohn
## Question 3 
![462537651_1056169252955195_3789763731896617641_n](https://github.com/user-attachments/assets/c649735d-5dc3-49c5-abc8-c33bce19aeff)
## Answer 
$Y = e^{Z} \Rightarrow \ln{Y} = Z$  
$F_Y(y) = P(Y \leq y) = P(e^Z \leq y) = P(Z \leq \ln{y})$   
Since, $Z \sim N(\mu, \sigma^2)$   
We can know that $F_Y(y) = \Phi\left(\frac{\ln(y) - \mu}{\sigma}\right)$  
We know that $f_Y(y) = \frac{d}{dy} F_Y(y)$  
by chain rule $f_Y(y) = \left[ \Phi\left(\frac{\ln(y) - \mu}{\sigma}\right) \right]' \left(\frac{\ln(y) - \mu}{\sigma}\right)' = \phi\left(\frac{\ln(y) - \mu}{\sigma}\right) \left(\frac{1}{\sigma y}\right)$   
=> $f_Y(y)= \frac{1}{2\pi} e^{-\frac{1}{2} \left(\frac{\ln(y) - \mu}{\sigma}\right)^2} \cdot \frac{1}{\sigma y}$
## Question 4
![462536868_1265152037837894_427853050666954556_n](https://github.com/user-attachments/assets/cbb2e977-113e-499e-9ac3-7f74874a1f1a)
## Answer 
$X \sim G(\alpha, \lambda)$ Thus, we can know that $f_X(x) = \frac{\lambda^{\alpha} x^{\alpha - 1} e^{-\lambda x}}{\Gamma(\alpha)} \quad \text{for } x \geq 0$    
=> $F_Y(y) = P(Y \leq y) = P(cX \leq y) = P(X \leq \frac{y}{c}) = F_X\left(\frac{y}{c}\right)$   
$f_Y(y) = \frac{d}{dy} F_Y(y) = \frac{d}{dy} F_X\left(\frac{y}{c}\right)$  
By chain rule, $\left[F_X\left(\frac{y}{c}\right)\right]' \cdot \frac{d}{dy}\left(\frac{y}{c}\right)$ = $\frac{1}{c} f_X\left(\frac{y}{c}\right)$  
Thus, $f_Y(y) = \frac{1}{c} \cdot \frac{\lambda^{\alpha}}{\Gamma(\alpha)} \left(\frac{y}{c}\right)^{\alpha - 1} e^{-\lambda \frac{y}{c}}$ $= \frac{\left(\frac{\lambda}{c}\right)^{\alpha}}{\Gamma(\alpha)} y^{\alpha - 1} e^{-y\left(\frac{\lambda}{c}\right)}$  
we can know that $Y \sim G\left(\alpha, \frac{\lambda}{c}\right)$ under Y=cX  
Therefore, we can prove that only $\lambda$ is affected by the transformation.
## Question 5
![462563992_937186478447463_3342444918834671733_n](https://github.com/user-attachments/assets/30134947-e388-4d99-b17b-4cc34e9628cb)
## Answer
### a. 
Given $a = 5, \quad c = 3, \quad m = 16, \quad X_0 = 7$  
The formula would be $X_n = (5X_{n-1} + 3) \mod 16$, and we can have following number:  
$X_0 = 7$  
$X_1 = 6$  
$X_2 = 1$  
$X_3 = 8$  
$X_4 = 11$  
$X_5 = 10$  
$X_6 = 5$  
$X_7 = 12$   
It seems  that it's random. However, due to m=16, the value of this case only between 1 to 15.  
Thus, it would finally repeat.  
### b.
(1) Given $a = 69069, \quad c = 0, \quad m = 2^{31}, $  
$X_0 = 69069$  
$X_1 = 475559465$  
$X_2 = 654291925$  
$X_3 = 1790562961$  
$X_4 = 957348637$  
$X_5 = 2091487033$  
$X_6 = 2135332261$  
$X_7 = 381957665$  
$X_8 = 1744831853$  
$X_9 = 1303896393$  
(2) Given $a = 65539, \quad c = 0, \quad m = 2^{31}, $ (RANDU)  
$X_0 = 65539$  
$X_1 = 393225$  
$X_2 = 1769499$  
$X_3 = 7077969$   
$X_4 = 26542323$  
$X_5 = 95552217$   
$X_6 = 334432395$  
$X_7 = 1146624417$   
$X_8 = 1722371299$  
$X_9 = 14608041$   
It seems that it is random but it still have some problem. And RANDU are known to have serious flaws.  
## Question 6 
![462547299_1517445808959769_8127828124782661964_n](https://github.com/user-attachments/assets/920c3ab6-f2b1-44d9-8b03-5fd5bbc60e80)
## Answer
$X_1$ = game won by player 1   
$X_2$ = game won by player 2   
$X_3$ = game won by player 3  
$X_1 + X_2 + X_3 = 10$  
probability of winning $p_1=p_2=p_3=\frac{1}{3}$  
Joint distribution: (follow multinomial distribution)  
$P(X_1 = k_1, X_2 = k_2, X_3 = k_3) = \frac{10!}{k_1! \, k_2! \, k_3!} \left(\frac{1}{3}\right)^{k_1} \left(\frac{1}{3}\right)^{k_2} \left(\frac{1}{3}\right)^{k_3}$  
where $k_1,k_2,k_3>0$ and $k_1 + k_2 + k_3 = 10$
## Question 7
![462541844_1936448073492469_337199694784007036_n](https://github.com/user-attachments/assets/fe3d9355-eeb9-4cc6-bbb8-f83cb1813a18)
## Answer
ellipse area = $\pi a b$  
$\int_{\text{ellipse}} f_{XY}(x, y) \, dA = 1$  
=> $f_{XY}(x, y)$ *ellipse area = 1  
=> $f_{XY}(x, y)$ = $\frac{1}{\pi a b}$ , $\frac{x^2}{a^2} + \frac{y^2}{b^2} \leq 1$  and  $f_{XY}(x, y)$ = 0, $\frac{x^2}{a^2} + \frac{y^2}{b^2} > 1$  
  
X marginal densities 
$\frac{x^2}{a^2} + \frac{y^2}{b^2} \leq 1$ => $y^2 \leq b^2 \left(1 - \frac{x^2}{a^2}\right)$  
=> $y \in \left[-b \sqrt{1 - \frac{x^2}{a^2}}, \, b \sqrt{1 - \frac{x^2}{a^2}}\right]$  
Thus, $f_X(x) = \int_{-b \sqrt{1 - \frac{x^2}{a^2}}}^{b \sqrt{1 - \frac{x^2}{a^2}}} \frac{1}{\pi a b} \ dy$  
=> $f_X(x) = \frac{2}{\pi a} \sqrt{1 - \frac{x^2}{a^2}}$ , $|x| \leq a$  

Y marginal densities 
$\frac{x^2}{a^2} + \frac{y^2}{b^2} \leq 1$ => $x^2 \leq a^2 \left(1 - \frac{x\y^2}{b^2}\right)$  
=> $x \in \left[-a \sqrt{1 - \frac{y^2}{b^2}}, \, a \sqrt{1 - \frac{y^2}{b^2}}\right]$  
Thus, $f_Y(y) = \int_{-a \sqrt{1 - \frac{y^2}{b^2}}}^{a \sqrt{1 - \frac{y^2}{b^2}}} \frac{1}{\pi a b} \ dy$  
=> $f_Y(y) = \frac{2}{\pi b} \sqrt{1 - \frac{y^2}{b^2}}$ , $|y| \leq b$
## Question 8
![462538184_1207808570484638_8996513959186368264_n](https://github.com/user-attachments/assets/6b342781-30e6-4fc7-b1ee-9a3e5ec854f5)
## Answer

