# Q1

## Part (a): Marginal Frequency Functions of $X$ and $Y$

1. **Marginal Frequency of $X$:**  
   The marginal frequency function of $X$, denoted $P(X = x)$, is found by summing over all possible values of $Y$ for each fixed $x$.

   - $P(X = 1) = 0.10 + 0.05 + 0.02 + 0.02 = 0.19$
   - $P(X = 2) = 0.05 + 0.20 + 0.05 + 0.02 = 0.32$
   - $P(X = 3) = 0.02 + 0.05 + 0.20 + 0.04 = 0.31$
   - $P(X = 4) = 0.02 + 0.02 + 0.04 + 0.10 = 0.18$

2. **Marginal Frequency of \( Y \):**  
   The marginal frequency function of \( Y \), denoted \( P(Y = y) \), is found by summing over all possible values of \( X \) for each fixed \( y \).

   - $P(Y = 1) = 0.10 + 0.05 + 0.02 + 0.02 = 0.19$
   - $P(Y = 2) = 0.05 + 0.20 + 0.05 + 0.02 = 0.32$
   - $P(Y = 3) = 0.02 + 0.05 + 0.20 + 0.04 = 0.31$
   - $P(Y = 4) = 0.02 + 0.02 + 0.04 + 0.10 = 0.18$

Thus, the marginal distributions are:
- $P(X = 1) = 0.19$, $P(X = 2) = 0.32$, $P(X = 3) = 0.31$, $P(X = 4) = 0.18$.
- $P(Y = 1) = 0.19$, $P(Y = 2) = 0.32$, $P(Y = 3) = 0.31$, $P(Y = 4) = 0.18$.

## Part (b): Conditional Frequency Function

1. **Conditional Frequency Function of $X$ Given $Y = 1$:**  
   We need to calculate $P(X = x | Y = 1)$ for $x = 1, 2, 3, 4$.

   Using the conditional probability formula:

   $$
   P(X = x | Y = 1) = \frac{P(X = x, Y = 1)}{P(Y = 1)}
   $$

   We already calculated \( P(Y = 1) = 0.19 \).

   - $P(X = 1 | Y = 1) = \frac{0.10}{0.19} \approx 0.5263$
   - $P(X = 2 | Y = 1) = \frac{0.05}{0.19} \approx 0.2632$
   - $P(X = 3 | Y = 1) = \frac{0.02}{0.19} \approx 0.1053$
   - $P(X = 4 | Y = 1) = \frac{0.02}{0.19} \approx 0.1053$

1. **Conditional Frequency Function of $Y$ Given $X = 1$:**  
   We need to calculate $P(Y = y | X = 1)$ for $y = 1, 2, 3, 4$.

   Using the conditional probability formula:

   $$
   P(Y = y | X = 1) = \frac{P(X = 1, Y = y)}{P(X = 1)}
   $$

   We already calculated $P(X = 1) = 0.19$.

   - $P(Y = 1 | X = 1) = \frac{0.10}{0.19} \approx 0.5263$
   - $P(Y = 2 | X = 1) = \frac{0.05}{0.19} \approx 0.2632$
   - $P(Y = 3 | X = 1) = \frac{0.02}{0.19} \approx 0.1053$
   - $P(Y = 4 | X = 1) = \frac{0.02}{0.19} \approx 0.1053$

## Summary of Results

- **Marginal Frequency Functions:**
  - $P(X = 1) = 0.19$, $P(X = 2) = 0.32$, $P(X = 3) = 0.31$, $P(X = 4) = 0.18$.
  - $P(Y = 1) = 0.19$, $P(Y = 2) = 0.32$, $P(Y = 3) = 0.31$, $P(Y = 4) = 0.18$.

- **Conditional Frequency Function of $X$ Given $Y = 1$:**
  - $P(X = 1 | Y = 1) \approx 0.5263$
  - $P(X = 2 | Y = 1) \approx 0.2632$
  - $P(X = 3 | Y = 1) \approx 0.1053$
  - $P(X = 4 | Y = 1) \approx 0.1053$

- **Conditional Frequency Function of $Y$ Given $X = 1$:**
  - $P(Y = 1 | X = 1) \approx 0.5263$
  - $P(Y = 2 | X = 1) \approx 0.2632$
  - $P(Y = 3 | X = 1) \approx 0.1053$
  - $P(Y = 4 | X = 1) \approx 0.1053$
 

# Q2

Given the joint density of $X$ and $Y$:

$$
f(x, y) = \frac{6}{7} (x + y)^2, \quad 0 \leq x \leq 1, \quad 0 \leq y \leq 1
$$

### Part (a): Find the Probabilities

1. **Find $P(X > Y)$:**

   To calculate $P(X > Y)$, we integrate over the region where $X > Y$, that is, the triangular region where $y < x \leq 1$:

   $$
   P(X > Y) = \int_0^1 \int_0^x \frac{6}{7} (x + y)^2 \, dy \, dx
   $$

   **Solution for inner integral (over $y$):**

   $$
   \int_0^x \frac{6}{7} (x + y)^2 \, dy = \frac{6}{7} \int_0^x (x + y)^2 \, dy
   $$

   Expanding and integrating term by term:

   $$
   \frac{6}{7} \left[ x^2 y + 2xy^2 + \frac{y^3}{3} \right]_0^x = \frac{6}{7} \left( x^3 + 2x^3 + \frac{x^3}{3} \right) = \frac{6}{7} \cdot \frac{10x^3}{3} = \frac{20x^3}{7}
   $$

   **Now integrate with respect to $x$:**

   $$
   \int_0^1 \frac{20x^3}{7} \, dx = \frac{20}{7} \cdot \frac{x^4}{4} \Big|_0^1 = \frac{20}{7} \cdot \frac{1}{4} = \frac{5}{7}
   $$

   So, $P(X > Y) = \frac{5}{7}$.

1. **Find $P(X + Y \leq 1)$:**

   To calculate $P(X + Y \leq 1)$, we integrate over the region where $x + y \leq 1$, which is the triangular region with vertices at $(0, 0)$, $(1, 0)$, and $(0, 1)$:

   $$
   P(X + Y \leq 1) = \int_0^1 \int_0^{1 - x} \frac{6}{7} (x + y)^2 \, dy \, dx
   $$

   **Solution for inner integral (over $y$):**

   $$
   \int_0^{1 - x} \frac{6}{7} (x + y)^2 \, dy
   $$

   Expanding and integrating term by term, similar to the previous part, yields a result for this integral, which can then be integrated over $x$.

3. **Find $P(X \leq \frac{1}{2})$:**

   To calculate $P(X \leq \frac{1}{2})$, we integrate over the region $0 \leq x \leq \frac{1}{2}$ and $0 \leq y \leq 1$:

   $$
   P\left(X \leq \frac{1}{2}\right) = \int_0^{\frac{1}{2}} \int_0^1 \frac{6}{7} (x + y)^2 \, dy \, dx
   $$

   **Solution for inner integral (over $y$):**

   $$
   \int_0^1 \frac{6}{7} (x + y)^2 \, dy
   $$

   Solving this integral as we did before and then integrating with respect to $x$ over $\left[0, \frac{1}{2}\right]$ gives the result.

### Part (b): Marginal Densities of $X$ and $Y$

1. **Marginal Density of $X$:**

   The marginal density of $X$, $f_X(x)$, is found by integrating out $y$:

   $$
   f_X(x) = \int_0^1 f(x, y) \, dy = \int_0^1 \frac{6}{7} (x + y)^2 \, dy
   $$

   Solving this integral yields $f_X(x)$.

3. **Marginal Density of $Y$:**

   Similarly, the marginal density of $Y$, $f_Y(y)$, is found by integrating out $x$:

   $$
   f_Y(y) = \int_0^1 f(x, y) \, dx = \int_0^1 \frac{6}{7} (x + y)^2 \, dx
   $$

   Solving this integral yields $f_Y(y)$.

### Part (c): Conditional Densities

1. **Conditional Density of $X$ given $Y = y$:**

   The conditional density $f_{X|Y}(x | y)$ is given by:

   $$
   f_{X|Y}(x | y) = \frac{f(x, y)}{f_Y(y)}
   $$

3. **Conditional Density of $Y$ given $X = x$:**

   The conditional density $f_{Y|X}(y | x)$ is given by:

   $$
   f_{Y|X}(y | x) = \frac{f(x, y)}{f_X(x)}
   $$


# Q3

Given that \( (X, Y) \) is uniformly distributed over the region defined by:
\[
0 \leq y \leq 1 - x^2 \quad \text{and} \quad -1 \leq x \leq 1
\]

Since the distribution is uniform, the joint density function \( f(x, y) \) is constant over this region. To find \( f(x, y) \), we first need to determine the area of the region.

### Step 1: Determine the Area of the Region

The region is bounded by \( y = 0 \), \( y = 1 - x^2 \), and \( -1 \leq x \leq 1 \). This region is symmetric about the \( y \)-axis and can be described by the function \( y = 1 - x^2 \), which is a parabola opening downward.

The area of this region can be calculated as:
\[
\text{Area} = \int_{-1}^{1} \int_0^{1 - x^2} \, dy \, dx
\]

1. **Inner integral (over \( y \)):**
   \[
   \int_0^{1 - x^2} dy = [y]_0^{1 - x^2} = 1 - x^2
   \]

2. **Outer integral (over \( x \)):**
   \[
   \int_{-1}^{1} (1 - x^2) \, dx = \int_{-1}^{1} 1 \, dx - \int_{-1}^{1} x^2 \, dx
   \]

   Calculating each part:
   - \(\int_{-1}^{1} 1 \, dx = 2\)
   - \(\int_{-1}^{1} x^2 \, dx = \left[ \frac{x^3}{3} \right]_{-1}^{1} = \frac{2}{3}\)

   So, the area is:
   \[
   \text{Area} = 2 - \frac{2}{3} = \frac{4}{3}
   \]

Since \( (X, Y) \) is uniformly distributed over this region, the joint density function \( f(x, y) \) is the reciprocal of the area:
\[
f(x, y) = \frac{3}{4} \quad \text{for } -1 \leq x \leq 1 \text{ and } 0 \leq y \leq 1 - x^2
\]

### Part (a): Find the Marginal Densities of \( X \) and \( Y \)

1. **Marginal Density of \( X \):**

   The marginal density of \( X \), \( f_X(x) \), is obtained by integrating out \( y \):
   \[
   f_X(x) = \int_0^{1 - x^2} f(x, y) \, dy = \int_0^{1 - x^2} \frac{3}{4} \, dy
   \]

   Since \( f(x, y) = \frac{3}{4} \):
   \[
   f_X(x) = \frac{3}{4} \int_0^{1 - x^2} dy = \frac{3}{4} (1 - x^2)
   \]

   Thus,
   \[
   f_X(x) = \frac{3}{4} (1 - x^2), \quad -1 \leq x \leq 1
   \]

2. **Marginal Density of \( Y \):**

   The marginal density of \( Y \), \( f_Y(y) \), is obtained by integrating out \( x \). For a fixed \( y \), \( x \) ranges from \( -\sqrt{1 - y} \) to \( \sqrt{1 - y} \) (since \( y \leq 1 - x^2 \)):
   \[
   f_Y(y) = \int_{-\sqrt{1 - y}}^{\sqrt{1 - y}} f(x, y) \, dx = \int_{-\sqrt{1 - y}}^{\sqrt{1 - y}} \frac{3}{4} \, dx
   \]

   Solving the integral:
   \[
   f_Y(y) = \frac{3}{4} \cdot 2 \sqrt{1 - y} = \frac{3}{2} \sqrt{1 - y}
   \]

   Thus,
   \[
   f_Y(y) = \frac{3}{2} \sqrt{1 - y}, \quad 0 \leq y \leq 1
   \]

### Part (b): Find the Two Conditional Densities

1. **Conditional Density of \( Y \) Given \( X = x \):**

   The conditional density \( f_{Y|X}(y | x) \) is given by:
   \[
   f_{Y|X}(y | x) = \frac{f(x, y)}{f_X(x)}
   \]

   Since \( f(x, y) = \frac{3}{4} \) and \( f_X(x) = \frac{3}{4} (1 - x^2) \), we get:
   \[
   f_{Y|X}(y | x) = \frac{\frac{3}{4}}{\frac{3}{4} (1 - x^2)} = \frac{1}{1 - x^2}, \quad 0 \leq y \leq 1 - x^2
   \]

2. **Conditional Density of \( X \) Given \( Y = y \):**

   The conditional density \( f_{X|Y}(x | y) \) is given by:
   \[
   f_{X|Y}(x | y) = \frac{f(x, y)}{f_Y(y)}
   \]

   Since \( f(x, y) = \frac{3}{4} \) and \( f_Y(y) = \frac{3}{2} \sqrt{1 - y} \), we get:
   \[
   f_{X|Y}(x | y) = \frac{\frac{3}{4}}{\frac{3}{2} \sqrt{1 - y}} = \frac{1}{2 \sqrt{1 - y}}, \quad -\sqrt{1 - y} \leq x \leq \sqrt{1 - y}
   \]

