##Q1
gamma function is defined as

$$
\Gamma(x) = \int_0^\infty x^{u-1} e^{-u} \, du \quad , \quad x,u > 0
$$

a) 

$$
\Gamma(1) = \int_0^\infty u^0 e^{-u} \, du
$$

$$
= \int_0^\infty e^{-u} \, du
$$

$$
= -e^{-u} \Big|_0^\infty
$$

$$
= -e^{-\infty} - (-e^0)
$$

$$
= 0 + 1
$$

b) 

$$
\text{LHS} = \Gamma(x+1) = \int_0^\infty u^x e^{-u} \, du
$$

let $I = \int u^x e^{-u} \, du$ is the corresponding indefinite integral

$$
I = u^x (-e^{-u}) - \int x u^{x-1} (-e^{-u}) \, du
$$

$$
= -u^x e^{-u} + x \int u^{x-1} e^{-u} \, du
$$

$$
I_0^\infty = (-u^x e^{-u}) \Big|_0^\infty + x \int_0^\infty u^{x-1} e^{-u} \, du
$$

$$
= 0 + x \cdot \Gamma(x) = \text{RHS}
$$

c) using the result of part (b)

$$
\Gamma(n) = (n-1)\Gamma(n-1)
$$

$$
= (n-1)\left[ (n-2)\Gamma(n-2) \right]
$$

$$
= (n-1)n-2\left[ (n-3)\Gamma(n-3) \right]
$$

$$
\vdots
$$

$$
= (n-1)(n-2)(n-3)\cdots \Gamma(1)
$$

$$
[\text{For } n \in \mathbb{N}, \text{ since } n > 0]
$$

$$
= (n-1)(n-2)(n-3)\cdots 1 \quad [\Gamma(1)=1 \text{ from part (a)}]
$$

$$
= (n-1)!
$$

$$
\therefore \Gamma(n) = (n-1)! \text{ for } n = 1,2,3,\dots \quad (n \in \mathbb{N})
$$


##Q2
### Explanation

in this question we have to show that the normal density integrates to 1 and  
it is given that

$$
\int_{-\infty}^{\infty} \exp\left(-\frac{x^2}{2}\right) dx = \sqrt{2\pi}
$$

squaring both sides and re-express the problem as that of showing

$$
\left( \int_{-\infty}^{\infty} \exp\left(-\frac{x^2}{2}\right) dx \right) \left( \int_{-\infty}^{\infty} \exp\left(-\frac{y^2}{2}\right) dy \right) = 2\pi
$$

---

### Step 1 of 2

if $X \sim N(\mu, \sigma^2)$, then its pdf is:

$$
f_X(x) = \frac{1}{\sigma \sqrt{2\pi}} \exp\left(-\frac{(x-\mu)^2}{2\sigma^2}\right)
$$

where, $\mu \in \mathbb{R}, \sigma > 0$ and $X \in \mathbb{R}$.

we have to show

$$
\int_{-\infty}^{\infty} f_X(x) dx = 1.
$$

firstly let's prove the lemma:

**Lemma:**

$$
\int_{-\infty}^{\infty} \exp\left(-\frac{x^2}{2}\right) dx = \sqrt{2\pi}
$$

let's denote the integral on the left side as $I$. instead of calculating $I$, we'll calculate $I^2$.

as the function under the integral is always strictly positive, we can apply fubini's theorem:

$$
I^2 = \left( \int_{-\infty}^{\infty} \exp\left(-\frac{x^2}{2}\right) dx \right) \cdot \left( \int_{-\infty}^{\infty} \exp\left(-\frac{y^2}{2}\right) dy \right)
$$

$$
= \int_{-\infty}^{\infty} \int_{-\infty}^{\infty} \exp\left( -\frac{x^2 + y^2}{2} \right) dxdy
$$

$$
= \int_{-\infty}^{\infty} \int_{-\infty}^{\infty} \exp\left( -\frac{r^2}{2} \right) dxdy
$$

$$
= \left[ \begin{aligned}
x &= r\cos\varphi \\
y &= r\sin\varphi \\
J &= \begin{vmatrix} \cos\varphi & -r\sin\varphi \\ \sin\varphi & r\cos\varphi \end{vmatrix} = r \\
x^2 + y^2 &= r^2
\end{aligned} \right]
$$

$$
= \int_0^{2\pi} \int_0^{\infty} \exp\left(-\frac{r^2}{2}\right) rdrd\varphi
$$

$$
= \left[ \begin{aligned}
t &= \frac{r^2}{2} \quad r = 0 \Rightarrow t = 0 \\
dt &= r \, dr \quad r = +\infty \Rightarrow t = +\infty
\end{aligned} \right]
$$

$$
= \int_0^{2\pi} \int_0^{\infty} \exp(-t) dtd\varphi
$$

$$
= \int_0^{2\pi} \left[ -\exp(-t)\Big|_0^{\infty} \right] d\varphi
$$

$$
= \int_0^{2\pi} (0 - 1) d\varphi
$$

$$
= \int_0^{2\pi} 1 d\varphi
$$

$$
= 2\pi
$$

hence, the square root of $I^2$ yields:

$$
I = \sqrt{2\pi}
$$

---

### Step 2 of 2

now get returning to our initial statement:

$$
\int_{-\infty}^{\infty} f_X(x) = \int_{-\infty}^{\infty} \frac{1}{\sigma\sqrt{2\pi}} \exp\left(-\frac{(x-\mu)^2}{2\sigma^2}\right) dx
$$

$$
= \frac{1}{\sqrt{2\pi}} \int_{-\infty}^{\infty} \exp\left(-\frac{(x-\mu)^2}{2\sigma^2}\right) dx
$$

$$
= \frac{1}{\sqrt{2\pi}} \int_{-\infty}^{\infty} \exp\left(-\frac{y^2}{2}\right) dy \quad \left[ \begin{aligned}
y &= \frac{x-\mu}{\sigma} \quad x = -\infty \Rightarrow y = -\infty \\
dy &= \frac{1}{\sigma} dx \quad x = +\infty \Rightarrow y = +\infty
\end{aligned} \right]
$$

$$
= \frac{1}{\sqrt{2\pi}} \int_{-\infty}^{\infty} \exp\left(-\frac{y^2}{2}\right) dy
$$

$$
= \frac{1}{\sqrt{2\pi}} \cdot \sqrt{2\pi}
$$

$$
= 1.
$$

##Q3
