# Q2
## Find the Mean and Variance of a Expotential
by Angela   https://youtu.be/M76qBTuLMo4

An Exponential random variable $\(X\)$ has the following probability density function (PDF):

$$
f(x) = 
\begin{cases}
\lambda e^{-\lambda x}, & \text{when } x \geq 0, \\
0, & \text{when } x < 0,
\end{cases}
$$

where $\lambda\$ is the rate parameter, $\lambda > 0$.

---

### Mean $\(E(X)\)$

We know that the **mean** of a random variable is

$$
E(X) = \int_{-\infty}^\infty x f(x) dx
$$

#### Step 1: Simplify the integral

Since $f(x) = 0$ for $x < 0$ and  $f(x) = \lambda e^{-\lambda x}$ for $x \geq 0$, the integral becomes:

$$
E(X) = \int_{0}^\infty x \lambda e^{-\lambda x} dx
$$

#### Step 2: Solve the integral

$$
\begin{aligned}
E(X) &= \int_{0}^\infty x \lambda e^{-\lambda x} dx, \quad \text{by integral by part, let } u = x,  du = dx,  dv = \lambda e^{-\lambda x} dx,  v = -e^{-\lambda x} \\
&= -xe^{-\lambda x}\Big|^\infty\_0 + \int_{0}^\infty e^{-\lambda x} dx \\
&= 0 - \frac{1}{\lambda} e^{-\lambda x}\Big|_0^\infty\\
&= -(0-\frac{1}{\lambda})\\
&=\frac{1}{\lambda}
\end{aligned}
$$

Thus:

$$
E(X) = \frac{1}{\lambda}
$$

---

### Variance $(\text{Var}(X)\)$

We know that the **variance** of a random variable is 

$$
\text{Var}(X) = E(X^2) - [E(X)]^2
$$

and

$$
E(X^2) = \int_{-\infty}^\infty x^2 f_X(x) dx
$$

#### Step 1: Compute $E(X^2)$

Simplify the integral

Since $f(x) = 0$ for $x < 0$ and  $f(x) = \lambda e^{-\lambda x}$ for $x \geq 0$, the integral becomes:

$$
E(X^2) = \int_{0}^\infty x^2 \lambda e^{-\lambda x} dx
$$

Solve the integral

$$
\begin{aligned}
E(X^2) &= \int_{0}^\infty x^2 \lambda e^{-\lambda x} dx, \quad \text{by integral by part, let } u = x^2,  du = 2xdx,  dv = \lambda e^{-\lambda x} dx,  v = -e^{-\lambda x} \\
&= -x^2e^{-\lambda x}\Big|^\infty\_0 + \int_{0}^\infty 2xe^{-\lambda x} dx \\
&= 0 + \int_{0}^\infty 2xe^{-\lambda x} dx,\quad \text{by integral by part, let } u = 2x,  du = 2dx,  dv = e^{-\lambda x} dx,  v = -\frac{1}{\lambda}e^{-\lambda x} \\
&= -2xe^{-\lambda x}\Big|^\infty\_0 + \int_{0}^\infty \frac{2}{\lambda}e^{-\lambda x} dx \\
&=\frac{2}{\lambda^2}e^{-\lambda x}\Big|^\infty\_0\\
&=0-(0-\frac{2}{\lambda^2})\\
&=\frac{2}{\lambda^2}
\end{aligned}
$$

#### Step 2: Substitute into the variance formula

Now we know: $E(X^2) = \frac{2}{\lambda^2}$, and $E(X) = \frac{1}{\lambda}.$

Substitute these into the variance formula:

$$
\text{Var}(X) = \frac{2}{\lambda^2} - \left(\frac{1}{\lambda}\right)^2
$$

Simplify:

$$
\text{Var}(X) = \frac{2}{\lambda^2} - \frac{1}{\lambda^2}
$$

$$
\text{Var}(X) = \frac{1}{\lambda^2}
$$

---

### Final Results

1. **Mean**:

$$
E(X) = \frac{1}{\lambda}
$$

2. **Variance**:

$$
\text{Var}(X) = \frac{1}{\lambda^2}
$$


