# 4.43

## Problem:
Show that:
$\text{Var}(X - Y) = \text{Var}(X) + \text{Var}(Y) - 2\text{Cov}(X, Y).$

---

## Solution:

### Step 1: Recall the definition of variance
The variance of a random variable $Z$ is defined as:

$\text{Var}(Z) = E[Z^2] - (E[Z])^2.$

Here, $Z = X - Y$, so we can write:

$\text{Var}(X - Y) = E[(X - Y)^2] - [E(X - Y)]^2.$

---

### Step 2: Expand $(X - Y)^2$
Expand the square term:

$(X - Y)^2 = X^2 - 2XY + Y^2.$

Take the expectation:

$E[(X - Y)^2] = E(X^2) - 2E(XY) + E(Y^2).$

Now, rewrite the variance:

$\text{Var}(X - Y) = \big[E(X^2) - 2E(XY) + E(Y^2)\big] - \big[E(X - Y)\big]^2.$

---

### Step 3: Break down $E(X - Y)$
Using the linearity of expectation:

$E(X - Y) = E(X) - E(Y).$

So:

$[E(X - Y)]^2 = [E(X) - E(Y)]^2.$

Substitute this into the variance equation:

$\text{Var}(X - Y) = \big[E(X^2) - 2E(XY) + E(Y^2)\big] - [E(X) - E(Y)]^2.$

---

### Step 4: Relate to variance and covariance
Recall the definitions of variance and covariance:
1. Variance:

   $\text{Var}(X) = E(X^2) - [E(X)]^2, \quad \text{Var}(Y) = E(Y^2) - [E(Y)]^2.$

3. Covariance:

   $\text{Cov}(X, Y) = E(XY) - E(X)E(Y).$

Using these definitions:
- $E(X^2) = \text{Var}(X) + [E(X)]^2$,
- $E(Y^2) = \text{Var}(Y) + [E(Y)]^2$,
- $E(XY) = \text{Cov}(X, Y) + E(X)E(Y)$.

---

### Step 5: Substitute into the variance equation
Substitute $E(X^2)$, $E(Y^2)$, and $E(XY)$ into:

$\text{Var}(X - Y) = \big[E(X^2) - 2E(XY) + E(Y^2)\big] - [E(X) - E(Y)]^2.$

1. Substitute $E(X^2)$ and $E(Y^2)$:

   $\text{Var}(X - Y) = \big[\text{Var}(X) + [E(X)]^2 - 2(E(XY)) + \text{Var}(Y) + [E(Y)]^2\big] - [E(X) - E(Y)]^2.$

3. Substitute $E(XY)$:

   $\text{Var}(X - Y) = \text{Var}(X) + [E(X)]^2 - 2[\text{Cov}(X, Y) + E(X)E(Y)] + \text{Var}(Y) + [E(Y)]^2 - [E(X) - E(Y)]^2.$

5. Simplify $[E(X) - E(Y)]^2$:

   $[E(X) - E(Y)]^2 = [E(X)]^2 - 2E(X)E(Y) + [E(Y)]^2.$

7. Subtract $[E(X) - E(Y)]^2$ from the rest:

   $\text{Var}(X - Y) = \text{Var}(X) + \text{Var}(Y) - 2\text{Cov}(X, Y).$

---

## Final Answer:
We have shown that:

$\text{Var}(X - Y) = \text{Var}(X) + \text{Var}(Y) - 2\text{Cov}(X, Y).$

---

## Explanation:
1. The key idea is to expand $(X - Y)^2$ and use the linearity of expectation.
2. By substituting the definitions of variance and covariance, we simplify the expanded terms.
3. This formula is useful because it relates the variance of a difference to the variances and covariance of the individual random variables.
