# 01_Rix

by 周子揚 Rix

## Q1. 

### Questions 

![image](https://github.com/user-attachments/assets/da5121e5-c2f3-465b-b660-3fae5ef5c0a5)

### Answers

![image](https://github.com/user-attachments/assets/596eaf6e-e024-49ac-aa22-e77fd3a0a62a)

## Q2. 

### Questions 

![image](https://github.com/user-attachments/assets/9e60fe51-d6a2-4861-af57-f14c9d81b8a0)

### Answers

![image](https://github.com/user-attachments/assets/0ebcec01-83bd-46f0-9add-d2a53c4565a9)

## Q3. 

### Questions 

![image](https://github.com/user-attachments/assets/fe23c9b6-a147-49b2-b981-28c7e33f9d10)


### Answers

![image](https://github.com/user-attachments/assets/8b347975-f290-42f4-a2d3-2fe2a4d8760d)

## Q4. 

### Questions 

![image](https://github.com/user-attachments/assets/01bbe703-1662-4652-8b4f-0f5f99fe7169)


### Answers

![image](https://github.com/user-attachments/assets/dc3be8ee-25c4-454f-ab2c-5786b094361d)

## Q5. 

### Questions 

![image](https://github.com/user-attachments/assets/70b433ea-6bea-4858-8898-4f6ee61dd02c)

### Answers

proof  
$$P(Z ≤ z) = P(F(X) ≤ z) = P(X ≤ F^{−1}(z)) = F(F^{−1}(z)) = z$$  
This is the uniform cdf.

## Q6. 

### Questions 

![image](https://github.com/user-attachments/assets/f2de8cb7-45c8-4e94-91f6-cc00cd5c1e7c)

### Answers

proof  
$$P(X ≤ x) = P(F^{−1}(U) ≤ x) = P(U ≤ F(x)) = F(x)$$  

## Q7. 

### Questions 

![image](https://github.com/user-attachments/assets/e797b0b8-5478-4464-b3c7-a383d617aa7f)

### Answers

![image](https://github.com/user-attachments/assets/72887eb8-8ac4-4da6-85d2-191be1daf42d)
