## Q1

**Show that if $X \sim F_{n,m} \), then \( X^{-1} \sim F_{m,n}$.**

---

## Solution

### Step 1: Given Information

It is given that $X \sim F_{n,m}$.

The probability density function (PDF) of $X$ is:

$f_X(x) = \frac{1}{B\left( \frac{n}{2}, \frac{m}{2} \right)} \left( \frac{n}{m} \left( \frac{n}{m} x \right)^{\frac{n}{2} - 1} \right) \left( 1 + \frac{n}{m} x \right)^{-\frac{n+m}{2}}, \quad 0 < x < \infty.$

Let $Y = \frac{1}{X} \), where \( g(x) = \frac{1}{x}$.

The inverse function $g^{-1}(y)$ is:

$g^{-1}(y) = \frac{1}{y}.$

The derivative of $g^{-1}(y)$ is:

$\frac{d}{dy} \left( g^{-1}(y) \right) = -\frac{1}{y^2}.$

---

### Step 2: Deriving the PDF of $Y$

The PDF of $Y$ is given by the transformation of variables formula:

$f_Y(y) = f_X\left( g^{-1}(y) \right) \cdot \left| \frac{d}{dy} g^{-1}(y) \right|.$

Substitute $X = g^{-1}(y) = \frac{1}{y}$:

$f_Y(y) = f_X\left( \frac{1}{y} \right) \cdot \left| -\frac{1}{y^2} \right|.$

Simplify step by step:

1. Substitute $f_X(x)$ into $f_Y(y)$:

$f_Y(y) = \frac{1}{B\left( \frac{n}{2}, \frac{m}{2} \right)} \left( \frac{n}{m} \left( \frac{n}{m} \cdot \frac{1}{y} \right)^{\frac{n}{2} - 1} \right) \left( 1 + \frac{n}{m} \cdot \frac{1}{y} \right)^{-\frac{n+m}{2}} \cdot \frac{1}{y^2}.$

2. Simplify the terms:

$f_Y(y) = \frac{1}{B\left( \frac{n}{2}, \frac{m}{2} \right)} \cdot \left( \frac{m}{n} \right)^{\frac{n}{2}} \cdot y^{-\frac{n}{2} - 1} \left( 1 + \frac{m}{n} y \right)^{-\frac{n+m}{2}}.$

3. Recognize the resulting PDF matches that of $F_{m,n}$:

$f_Y(y) = \frac{1}{B\left( \frac{m}{2}, \frac{n}{2} \right)} \left( \frac{m}{n} \right)^{\frac{m}{2}} y^{\frac{m}{2} - 1} \left( 1 + \frac{m}{n} y \right)^{-\frac{m+n}{2}}.$

---

### Conclusion

The derived PDF of $Y = X^{-1}$ is the PDF of $F_{m,n}$. Therefore:

$X^{-1} \sim F_{m,n}.$

---

## Q2

**Show that if $T \sim t_n$, then $T^2 \sim F_{1,n}$.**

---

## Solution

To show this relationship, we need to understand the properties of the $t$-distribution and the $F$-distribution.

### Background: $t$-distribution and $F$-distribution

1. **$t$-distribution**:
   - The $t$-distribution arises when estimating the mean of a normally distributed population with small sample sizes or unknown population standard deviation.
   - It is characterized by its **degrees of freedom** $n$ and has a symmetric bell-shaped curve similar to the normal distribution.

2. **$F$-distribution**:
   - The $F$-distribution arises when comparing the variances of two populations.
   - It is characterized by its **degrees of freedom** $(df_1, df_2)$ and has a **right-skewed** curve.

---

### Step 1: Relationship between $T$ and $T^2$

Let $T \sim t_n$. By definition:
- $T$ follows a $t$-distribution with $n$ degrees of freedom.

When we **square $T$**, we get $T^2$. To determine the distribution of $T^2$, we use the formula for the $F$-distribution:

$F = \frac{(T^2 / df_1)}{1 + (T^2 / df_2)}.$

---

### Step 2: Substitution of Degrees of Freedom

Here:
- $df_1 = 1$ (numerator degrees of freedom),
- $df_2 = n$ (denominator degrees of freedom).

Substitute these values into the formula:

$F = \frac{(T^2 / 1)}{1 + (T^2 / n)}.$

Simplify the expression:

$F = \frac{T^2}{1 + \left( \frac{T^2}{n} \right)}.$

---

### Step 3: Identifying the Distribution

This expression confirms that $T^2$ follows an $F$-distribution with:
- **1 numerator degree of freedom**,
- **\( n \) denominator degrees of freedom**.

---

### Conclusion

Therefore:

$T^2 \sim F_{1,n} \quad \text{if} \quad T \sim t_n.$

---

## Q3

**Show that the Cauchy distribution and the $t$-distribution with 1 degree of freedom are the same.**

---

## Solution

### Step 1: Student $t$-Distribution

The probability density function (PDF) of the **Student $t$-distribution** with $\nu$ degrees of freedom is given as:


$f(x) = \frac{\Gamma\left( \frac{\nu + 1}{2} \right)}{\sqrt{\nu \pi} \, \Gamma\left( \frac{\nu}{2} \right)} \left( 1 + \frac{x^2}{\nu} \right)^{-\frac{\nu + 1}{2}}, \quad x \in \mathbb{R}. \tag{1}$

Here:
- $\nu$ represents the degrees of freedom.
- $\Gamma$ is the Gamma function.

---

### Step 2: Cauchy Distribution

The probability density function (PDF) of the **Cauchy distribution** is given as:

$f(x) = \frac{1}{\pi} \frac{1}{1 + x^2}, \quad x \in \mathbb{R}. \tag{2}$

---

### Step 3: Substitution $\nu = 1$ in the $t$-Distribution

Substitute $\nu = 1$ into equation (1) for the Student $t$-distribution:

$f(x) = \frac{\Gamma\left( \frac{1 + 1}{2} \right)}{\sqrt{1 \pi} \, \Gamma\left( \frac{1}{2} \right)} \left( 1 + \frac{x^2}{1} \right)^{-\frac{1 + 1}{2}}.$

Simplify the terms:
- $\frac{1 + 1}{2} = 1$,
- $\frac{x^2}{1} = x^2$,
- $\sqrt{1} = 1$.

Thus:

f(x) = \frac{\Gamma(1)}{\sqrt{\pi} \, \Gamma\left( \frac{1}{2} \right)} \left( 1 + x^2 \right)^{-1}.$

---

### Step 4: Gamma Function Values

From properties of the Gamma function:
- $\Gamma\left( \frac{1}{2} \right) = \sqrt{\pi}$,
- $\Gamma(1) = 1$.

Substitute these into the equation:

$f(x) = \frac{1}{\sqrt{\pi} \cdot \sqrt{\pi}} \cdot \frac{1}{1 + x^2}.$

Simplify:

$f(x) = \frac{1}{\pi} \cdot \frac{1}{1 + x^2}, \quad x \in \mathbb{R}.$

---

### Step 5: Comparison with Cauchy Distribution

The derived PDF matches exactly with the PDF of the Cauchy distribution (equation 2). Therefore, the **Student $t$-distribution** with 1 degree of freedom is identical to the **Cauchy distribution**.

---

## Conclusion

Thus, we have shown that:

$t_1 \sim \text{Cauchy Distribution}.$

$f(x) = \frac{1}{\pi} \frac{1}{1 + x^2}, \quad x \in \mathbb{R}.$

---

## Notes:
1. **Key Steps**:
   - Substitution $\nu = 1$ into the $t$-distribution formula.
   - Simplification using Gamma function properties.
2. **Cauchy Distribution**:
   - The Cauchy distribution is characterized by heavy tails and undefined mean/variance.
3. **Gamma Function**:
   - $\Gamma\left( \frac{1}{2} \right) = \sqrt{\pi}$ and $\Gamma(1) = 1$.

**Proved.**

---

## Q4

**Show that if $X$ and $Y$ are independent exponential random variables with $\lambda = 1$, then $Z = \frac{X}{Y}$ follows an $F$-distribution. 
Also, identify the degrees of freedom.**

---

## Solution

### Step 1: Given Information

1. $X$ and $Y$ are independent exponential random variables with rate parameter $\lambda = 1$.
2. The probability density functions (PDFs) of $X$ and $Y$ are:
   
   $f_X(x) = e^{-x}, \quad x \geq 0 \tag{1}$
   
   $f_Y(y) = e^{-y}, \quad y \geq 0. \tag{2}$

---

### Step 2: Deriving the PDF of $Z = \frac{X}{Y}$

To find the distribution of $Z = \frac{X}{Y}$, we start by considering the joint PDF of $X$ and $Y$, which are independent.

The PDF of $Z$ is given by:

$f_Z(z) = \int_0^\infty |y| f_X(zy) f_Y(y) \, dy.$

Substitute $f_X(x) = e^{-x}$ and $f_Y(y) = e^{-y}$ into the formula:

$f_Z(z) = \int_0^\infty y \cdot e^{-zy} \cdot e^{-y} \, dy \quad \text{(since \( x = zy \) and \( y > 0 \))}.$

Combine the exponents:

$f_Z(z) = \int_0^\infty y e^{-y(1 + z)} \, dy.$

---

### Step 3: Solving the Integral

The integral simplifies to:

$f_Z(z) = \int_0^\infty y e^{-y(1+z)} \, dy.$

Using the property of the **Gamma function**:

$\int_0^\infty y^{\alpha-1} e^{-\lambda y} \, dy = \frac{\Gamma(\alpha)}{\lambda^\alpha}, \quad \text{where} \, \alpha = 2, \, \lambda = 1 + z.$

Here:
- $\alpha = 2$ (since $y$ appears with a factor $y^1$),
- $\lambda = 1 + z$.

Thus:

$f_Z(z) = \frac{\Gamma(2)}{(1 + z)^2}.$

Simplify $\Gamma(2) = 1! = 1$:

$f_Z(z) = \frac{1}{(1 + z)^2}, \quad z > 0.$

---

### Step 4: Recognizing the $F$-Distribution

The PDF of the $F$-distribution with $d_1$ and $d_2$ degrees of freedom is:

$f(z) = \frac{1}{B\left( \frac{d_1}{2}, \frac{d_2}{2} \right)} \left( \frac{d_1}{d_2} \right)^{\frac{d_1}{2}} z^{\frac{d_1}{2} - 1} \left( 1 + \frac{d_1}{d_2} z \right)^{-\frac{d_1 + d_2}{2}}, \quad z > 0.$

When $d_1 = d_2 = 2$, the Beta function simplifies to $B(1, 1) = 1$, and the $F$-distribution reduces to:

$f(z) = \frac{1}{(1 + z)^2}.$

---

### Step 5: Conclusion

The derived PDF of $Z = \frac{X}{Y}$ matches the PDF of the $F$-distribution with:

- **2 numerator degrees of freedom** ($d_1 = 2$),
- **2 denominator degrees of freedom** ($d_2 = 2$).

Thus:

$Z = \frac{X}{Y} \sim F_{2,2}.$

---

## Summary

We have shown that if $X$ and $Y$ are independent exponential random variables with $\lambda = 1$, then $Z = \frac{X}{Y}$ follows an $F$-distribution with degrees of freedom $(2, 2)$.

$Z \sim F_{2,2}.$

---

## Q5



