## Q3 Find the mgf of the gamma distribution and use it to find its mean and variance
by Angela
### Moment-Generating Function
The probability density function of the gamma distribution is:

$$f(x) = \frac{\lambda^\alpha}{\Gamma(\alpha)} x^{\alpha-1} e^{-\lambda x}, \quad x \geq 0.$$

The mgf is defined as:

$$
M(t) = \mathbb{E}[e^{tX}] = \int_0^\infty e^{tx} f(x) \ dx.
$$

So the mgf of the gamma distribution is

$$
\begin{aligned}
M(t) &= \int_0^\infty e^{tx} \frac{\lambda^\alpha}{\Gamma(\alpha)} x^{\alpha-1} e^{-\lambda x} \ dx\\
&= \frac{\lambda^\alpha}{\Gamma(\alpha)} \int_0^\infty x^{\alpha-1} e^{-x(\lambda - t)} \ dx,\quad \text{let } u = -x(\lambda-t),  du = (\lambda-t)dx\\
&= \frac{\lambda^\alpha}{\Gamma(\alpha)} \int_0^\infty \frac{(\frac{u}{\lambda-t})^{\alpha-1}}{\lambda-t} e^{-u} \ du\\
&= \frac{\lambda^\alpha}{\Gamma(\alpha)} \int_0^\infty \frac{u^{\alpha-1}}{(\lambda-t)^\alpha} e^{-u} \ du\\
&= \frac{\lambda^\alpha}{\Gamma(\alpha)(\lambda-t)^\alpha} \int_0^\infty u^{\alpha-1} e^{-u} \ du,\quad \text{gamma function is defined as } \Gamma(\alpha)=\int_0^\infty u^{\alpha-1} e^{-u} \ du, \alpha>0\\
&= \frac{\lambda^\alpha}{\Gamma(\alpha)(\lambda-t)^\alpha}\Gamma(\alpha)\\
&= \frac{\lambda^\alpha}{(\lambda-t)^\alpha}
\end{aligned}
$$

### Mean and Variance
From the mgf:
1. **Mean**: The mean $\(E(X)\)$ is the first derivative of  $M(t)$ evaluated at $t = 0$:

$$
\begin{aligned}
M'(t) &= \frac{-\lambda^\alpha \cdot \alpha (\lambda-t)^{\alpha-1} \cdot (-1)}{(\lambda-t)^{2\alpha}} \\
&= \lambda^\alpha \cdot \alpha (\lambda-t)^{-\alpha-1} \\
&= \left(\frac{\lambda}{\lambda-t}\right)^\alpha \cdot \alpha \cdot \frac{1}{\lambda-t} \\
&= \alpha \frac{\lambda^\alpha}{(\lambda-t)^{\alpha+1}}
\end{aligned}
$$

At $t = 0$:

$$
M'(0) = \alpha \frac{\lambda^\alpha}{\lambda^{\alpha+1}} = \frac{\alpha}{\lambda} = \text{the mean of gamma dostribution}
$$

2. **Variance**: The second derivative of $M(t)$ at $t = 0$ gives $\mathbb{E}[X^2]$. Using:

$$
\begin{aligned}
M''(t) &= \alpha\lambda^\alpha \cdot \frac{(\alpha+1)(\lambda-t)^\alpha}{(\lambda-t)^{2\alpha+2}} \\
&= \frac{\alpha(\alpha+1)\lambda^\alpha}{(\lambda-t)^{\alpha+2}}
\end{aligned}
$$

evaluating at $t = 0$:

$$
M''(0) = \frac{\alpha(\alpha + 1)}{\lambda^2}.
$$

The variance is:

$$
\text{Var}(X) = \mathbb{E}[X^2] - (\mathbb{E}[X])^2 = \frac{\alpha(\alpha + 1)}{\lambda^2} - \left(\frac{\alpha}{\lambda}\right)^2 = \frac{\alpha}{\lambda^2}.
$$
