## Q49
![image](https://github.com/user-attachments/assets/1d81edde-a15b-48e4-9308-2a1d8b244af4)
  Gamma function is defined as:
  
  $\Gamma(x)$ = $\int_{0}^\infty u^{x-1}e^{-u}dx$

  a) $\Gamma(1)$ = $\int_{0}^\infty e^{-u}dx$ = $e^{-\infty} - (-e^0)$ = $1$

  b) 

  $LHS$ = $\Gamma(x+1)$ = $\int_{0}^\infty u^{x}e^{-u}dx$

  let $l$ = $\int_{0}^\infty u^{x}e^{-u}dx$ is the corresponding indefinite intergral

  $l$ = $u^{x}(-e^{-u})-\int xu^{x-1}(-e^{-u})du$

  = $-u^x e^{-u} + \int xu^{x-1}e^{-u}du$

  $l_{0}^{\infty}$ = $(-u^xe^{-u})]_0^{\infty} +x \times \int_0^{\infty} u^{x-1}e^{-u}du$

  = $0+\Gamma(x+1)$= $RHS$

  c) using the result of part b)

  $\Gamma(n)$ = $(n-1)\Gamma(n-1)$

  = $(n-1)[(n-2)\Gamma(n-2)]$

  = $(n-1)(n-2)[(n-3)\Gamma(n-3)]$

  = $(n-1)(n-2)(n-3)......\Gamma(1)$

  = $(n-1)!$

  d)

  $LHS$ = $(\frac{n}{2}-1)(\frac{n}{2}-2)(\frac{n}{2}-3)......\frac{1}{2}\Gamma(\frac{1}{2})$

  = $(\frac{n-2}{2})(\frac{n-4}{2})(\frac{n-6}{2})......\frac{1}{2}\sqrt{\pi}$

  = $\frac{\sqrt{\pi}}{2^{\frac{n-1}{2}}}[(n-2)(n-4)(n-6)......1]$

  = $\sqrt{\pi}2^{\frac{1-n}{2}}\frac{[(n-2)(n-4)(n-6......1\times(n-1)(n-3)......2)]}{(n-1)(n-3)(n-5)......2}$

  = $\frac{\sqrt{\pi}}{2^{\frac{n-1}{2}}}[\frac{(n-1)(n-2)(n-3)......1}{\frac{n-1}{2}\frac{n-3}{2}\frac{n-5}{2}......\frac{2}{2}2^{\frac{n-1}{2}}}]$

  = $\frac{\sqrt{\pi}}{2^{\frac{n-1}{2}}} \frac{(n-1)!}{(\frac{n-1}{2})(\frac{n-1}{2}-1)(\frac{n-1}{2}-2)......2^{\frac{n-1}{2}}}$

  = $\frac{\sqrt{\pi}}{2^{\frac{n-1}{2}}} \frac{(n-1)!}{(\frac{n-1}{2}!)}$ = $RHS$
  
## Q51
![image](https://github.com/user-attachments/assets/2c7532d1-6567-4754-8a78-4c9700dae275)


## Q53

## Q59

## Prove Proposition C

## Prove Proposition D

## Q65
