# Q3
## Identity  the bivaraite normal disitriubtion of page 14 of the slides in class

by Angela

We know that $$X_1$$ and $$X_2$$ are independent standard normal random vairables and that $$Y_1=X_1, Y_2=X_1+X_2$$.

So we can turn $$y_1=x_1, y_2=x_1+x_2$$ into $$x_1=y_1, x_2=-y_1+y_2$$.

Then calculate the Jacobian 

$$J=\left|
\begin{array}{cc}
\frac{dx_1}{dy_1} & \frac{dx_1}{dy_2} \\
\frac{dx_2}{dy_1} & \frac{dx_2}{dy_2} \\
\end{array}
\right|=\left|\begin{array}{cc}
1 & 0 \\
-1 & 1 \\
\end{array}
\right|=1$$

Since $$X_1$$ and $$X_2$$ are independent standard normal random variables,

$$f_{X_1, X_2}(x_1, x_2)=\frac{1}{2π}e^{-\frac{{x_1}^2+{x_2}^2}{2}} and\ x_1=y_1, x_2=-y_1+y_2$$ 

then

$$f_{Y_1, Y_2}(y_1, y_2)=f_{X_1, X_2}(y_1, y_2-y_2)·|J|=\frac{1}{2π}e^{-\frac{{y_1}^2+{y_2-y_1}^2}{2}}·|1|=\frac{1}{2π}e^{-\frac{2{y_1}^2-2y_1y_2+{y_2}^2}{2}}\ for\ -∞≤y_1, y_2≤∞$$

Compare it with the bivariate normal density function

$$f(y_1, y_2) = \frac{1}{2 \pi \sigma_{Y_1} \sigma_{Y_2} \sqrt{1 - \rho^2}} \cdot e^{ -\frac{1}{2(1 - \rho^2)} \left( \frac{(y_1 - \mu_{Y_1})^2}{\sigma_{Y_1}^2} + \frac{(y_2 - \mu_{Y_2})^2}{\sigma_{Y_2}^2} - \frac{2 \rho (y_1 - \mu_{Y_1})(y_2 - \mu_{Y_2})}{\sigma_{Y_1} \sigma_{Y_2}} \right)}\ for\-∞≤y_1, y_2≤∞$$

We can find that 

$$\sigma_{Y_1} \sigma_{Y_2}\sqrt{1 - \rho^2} = 1$$
$$(1 - \rho^2) \sigma_{Y_1}^2 = \frac{1}{2}$$
$$(1 - \rho^2) \sigma_{Y_2}^2 = 1$$
$$\frac{\rho}{(1 - \rho^2) \sigma_{Y_1} \sigma_{Y_2}} = 1$$

According to the above equation

$$\sqrt{1 - \rho^2}=\frac{1 - \rho^2}{\rho} ,\\rho=\frac{1}{\sqrt{2}}, so\ \sigma_{Y_1}=1\\ and\\ \sigma_{Y_2}=\sqrt{2}, Cov(Y_1, Y_2)=\rho\sigma_{Y_1} \sigma_{Y_2}=1$$

Thus
```math
(Y_1, Y_2) \sim N_2 \left( \begin{pmatrix} 0 \\ 0 \end{pmatrix}, \begin{pmatrix} 1 & 1 \\ 1 & 2 \end{pmatrix} \right)
```
