by Liza

## Question 9
Prove: P(A ∪ B) = P(A) + P(B) - P(A ∩ B)

## Solution
For any sets A and B, we have the disjoint union  
<br>
$A \cup B = (A \setminus B) \cup (A \cap B) \cup (B \setminus A)$

Then, by the third axiom  
<br>
$P(A \cup B) = P(A \setminus B) + P(A \cap B) + P(B \setminus A)$  
<br>
Since $P(A \setminus B) = P(A) - P(A \cap B)$ and $P(B \setminus A) = P(B) - P(B \cap A)$  
<br>
The result:  
<br>
$P(A \cup B) = P(A) - P(A \cap B) + P(A \cap B) + P(B) - P(B \cap A) = P(A) + P(B) - P(A \cap B)$





