## Question 3 
![462537651_1056169252955195_3789763731896617641_n](https://github.com/user-attachments/assets/c649735d-5dc3-49c5-abc8-c33bce19aeff)
## Answer 
$Y = e^{Z} \Rightarrow \ln{Y} = Z$  
$F_Y(y) = P(Y \leq y) = P(e^Z \leq y) = P(Z \leq \ln{y})$   
Since, $Z \sim N(\mu, \sigma^2)$   
We can know that $F_Y(y) = \Phi\left(\frac{\ln(y) - \mu}{\sigma}\right)$  
We know that $f_Y(y) = \frac{d}{dy} F_Y(y)$  
by chain rule $f_Y(y) = \left[ \Phi\left(\frac{\ln(y) - \mu}{\sigma}\right) \right]' \left(\frac{\ln(y) - \mu}{\sigma}\right)' = \phi\left(\frac{\ln(y) - \mu}{\sigma}\right) \left(\frac{1}{\sigma y}\right)$   
=> $f_Y(y)= \frac{1}{2\pi} e^{-\frac{1}{2} \left(\frac{\ln(y) - \mu}{\sigma}\right)^2} \cdot \frac{1}{\sigma y}$
