# HW0924byJohn
## Question 1 
![460218771_508470181988044_9073365785074834176_n (1)](https://github.com/user-attachments/assets/b2c87fe8-6d43-4e0f-8d64-f20d7818f9ca)
## Answer 
### a.
a red ball drawn from A then a red ball drawn from B: $$\frac{4}{9}$$ \* $$\frac{3}{10}$$= $$\frac{12}{90}$$  
a non-red ball drawn from A then a red ball drawn from B: $$\frac{5}{9}$$ \* $$\frac{2}{10}$$= $$\frac{10}{90}$$  
proability of a red ball drawn from B: $$\frac{12}{90}$$ + $$\frac{10}{90}$$= $$\frac{22}{90}$$ = $$\frac{11}{45}$$
### b. 
P(red ball drawn from A | red ball drawn from B) = $$\frac{P(\text{a red ball drawn from } A  \cap \text{a red ball drawn from } B)}{ P(\text{a red ball drawn from } B)}$$  
=> $$\frac{\frac{12}{90}}{\frac{22}{90}}$$ = $$\frac{6}{11}$$
## Question 2
![460546281_840782197887546_482067095598502841_n](https://github.com/user-attachments/assets/bbbaa129-7de5-44da-bfbc-c50b851a1ceb)
## Answer 
### a.
P(two or more head |　at least one head) = $$\frac{P(\text{ two or more head} \cap \text{at least one head } )}{ P(\text{at least one head} )}$$  
=> $$\frac{\frac{4}{8}}{1-\frac{1}{8}}$$ = $$\frac{4}{7}$$ P(at least one head)=1-P(no head)
### b.
P(at least one tail)=1-P(no tail)=1- $$\frac{1}{8}$$= $$\frac{7}{8}$$
## Question 3
![460530669_1057279525948877_3035462176641943920_n](https://github.com/user-attachments/assets/dc6474db-ad8b-4a38-a728-57885b25dfcd)
![461534523_1450495998951823_335398748956609987_n](https://github.com/user-attachments/assets/45724ff8-696f-45ce-a46e-87835a10c772)
## Answer
for each student's proability of leave is $$\frac{1}{3}$$ and the proability of stay is $$\frac{2}{3}$$
base on the question, now teacher named Jason to stay  
it means that P(Drew leave | Jason stay)+P(Drew stay | Jason stay) should be 1  
=> $$\frac{P(\text{Drew leave} \cap \text{Jason stay} )}{ P(\text{Jason stay} )}$$ = $$\frac{\frac{1}{3} \* \frac{2}{3}}{\frac{2}{3}}$$ and $$\frac{P(\text{Drew stay} \cap \text{Jason stay} )}{ P(\text{Jason stay} )}$$ = $$\frac{\frac{2}{3} \* \frac{2}{3}}{\frac{2}{3}}$$  
=> $$\frac{1}{3}$$ + $$\frac{2}{3}$$ =1
Therefore, the proability of Drew leave while no matter Jason or Chris stay is still $$\frac{1}{3}$$
## Question 4
![460494975_2521427174734273_7078602795050187097_n](https://github.com/user-attachments/assets/6227e63d-f991-4e5d-875e-cec8497b9801)
## Answer
P(work)=1-P(not work)  
for top and buttom path P(work)= $$(1-p)^2$$ => P(not work) = 1- $$(1-p)^2$$
medium path  P(not work) = p  
full system P(not work) = $$(1-(1-p)^2)^2\*p$$ => P(work) = 1- $$(1-(1-p)^2)^2\*p$$
## Question 5
![461542089_3828603457457031_6455242258185925742_n](https://github.com/user-attachments/assets/eeaebe72-f649-4340-a01a-a47607b8c2a8)
## Answer
By Multinomial coefficients, coefficirnt = $$\Bigg( \frac{7}{223} \Bigg)$$  
$$\Bigg( \frac{7}{223} \Bigg)$$ = $$\frac{7}{2\!2\!3\!}$$ = 210
## Question 6
![460188023_1196313651632503_965397432060202974_n](https://github.com/user-attachments/assets/a195f5cc-0242-424e-8a12-ae7e7b3ab398)
## Answer
For at least one more king, we can use all event less the rest 4 cards with no kings.  
all event: $$\Bigg( \frac{51}{4} \Bigg)$$  
rest 4 cards no kings: $$\Bigg( \frac{48}{4} \Bigg)$$  
proability:1- $$\frac{\Bigg( \frac{48}{4} \Bigg)}{\Bigg( \frac{51}{4} \Bigg)}$$ &asymp; 0.22137
## Question 7
![461768779_453843467086454_8134805616700167117_n](https://github.com/user-attachments/assets/59f41936-7752-4abe-bf49-d07d0d77ccbc)
## Answer
all possible event: $$7^5$$  
no two people choose the same floor(choose by sequence): 7\*6\*5\*4\*3  
proability: $$\frac{7\*6\*5\*4\*3}{7^5}$$ &asymp; 0.15
## Question 8
### Prove: P(∅) = 0
## Answer
For any two mutually exclusive event A and B, P(A),P(B)≧ 0, we can know that P(A &#8746; B)=P(A)+P(B)  
Now the entire sample space S, P(S)=1  
The empty set ∅ means no outcome  
P(S)+P(∅)=P(S &#8746; ∅)=P(S)    
=>P(∅)=0
## Question 9
### Prove:  P(A ∪ B) = P(A) + P(B) - P(A ∩ B)
## Answer
Let A,B two event   
P(A-B) means part of A not overlap with B ; P(B-A) means part of B not overlap with A  
P(A)=P(A-B)+P(A &#8745; B) ; P(B)=P(B-A)+P(B &#8745; A)  
P(A ∪ B)=P(A-B)+P(B-A)+P(A &#8745; B)  
=>P(A ∪ B) = P(A) + P(B) - P(A ∩ B)
