# HW1022 Q6
22. Consider a Poisson process on the real line, and denote by N ( t 1 , t 2 ) the number
of events in the interval ( t 1 , t 2 ) . If t 0 < t 1 < t 2 , ﬁnd the conditional distribution of
N ( t 0 , t 1 ) given that N ( t 0 , t 2 ) = n. (Hint: Use the fact that the numbers of events
in disjoint subsets are independent.)


### Step 1: Definitions and Properties

1. **Poisson Process**: In a Poisson process with rate \( \lambda \), the number of events in any interval \( (a, b) \) follows a Poisson distribution:

$$
N(a, b) \sim \text{Poisson}(\lambda (b - a)).
$$

2. **Independence**: The number of events in disjoint intervals are independent. Therefore, if we consider the intervals \( (t_0, t_1) \) and \( (t_1, t_2) \), the number of events in these intervals will be independent.

### Step 2: Distribution of Events

Let N(t0, t1) = X  and N(t1, t2) = Y  .

From the properties of the Poisson process:

- 

$$
X \sim \text{Poisson}(\lambda(t_1 - t_0))
$$

- 

$$
Y \sim \text{Poisson}(\lambda(t_2 - t_1))
$$

The total number of events in the interval \( (t_0, t_2) \) is:

$$
N(t_0, t_2) = N(t_0, t_1) + N(t_1, t_2) = X + Y.
$$

### Step 3: Conditional Distribution

Given that \( N(t_0, t_2) = n \), we want to find the conditional distribution of \( X \):

$$
P(X = k | X + Y = n).
$$

Using the property of the Poisson process and the independence of \( X \) and \( Y \):

$$
P(X = k | X + Y = n) = \frac{P(X = k, Y = n - k)}{P(X + Y = n)}.
$$

### Step 4: Calculate Probabilities

The probabilities are given by:

$$
P(X = k) = \frac{(\lambda(t_1 - t_0))^k e^{-\lambda(t_1 - t_0)}}{k!},
$$

$$
P(Y = n - k) = \frac{(\lambda(t_2 - t_1))^{n - k} e^{-\lambda(t_2 - t_1)}}{(n - k)!}.
$$

Now the probability \( P(X + Y = n) \) is:

$$
P(X + Y = n) = \frac{(\lambda(t_2 - t_0))^n e^{-\lambda(t_2 - t_0)}}{n!}.
$$

### Step 5: Combine and Simplify

Thus,

$$
P(X = k | X + Y = n) = \frac{\frac{(\lambda(t_1 - t_0))^k e^{-\lambda(t_1 - t_0)}}{k!} \cdot \frac{(\lambda(t_2 - t_1))^{n - k} e^{-\lambda(t_2 - t_1)}}{(n - k)!}}{\frac{(\lambda(t_2 - t_0))^n e^{-\lambda(t_2 - t_0)}}{n!}}.
$$

This simplifies to:

$$
= \frac{n!}{k!(n-k)!} \cdot \frac{(t_1 - t_0)^k (t_2 - t_1)^{n-k}}{(t_2 - t_0)^n}.
$$

### Step 6: Identify the Conditional Distribution

This is the form of the binomial distribution. Therefore, we conclude:

$$
N(t_0, t_1) | N(t_0, t_2) = n \sim \text{Binomial}\left(n, \frac{t_1 - t_0}{t_2 - t_0}\right).
$$

### Final Result

The conditional distribution of \( N(t_0, t_1) \) given \( N(t_0, t_2) = n \) is:

$$
N(t_0, t_1) | N(t_0, t_2) = n \sim \text{Binomial}\left(n, \frac{t_1 - t_0}{t_2 - t_0}\right).
$$
